suite

modélisation Isabelle/HOModel.v
@@ -3,6 +3,8 @@ Require Import List.
 Require Import ListSet.
 Require Import Coq.Logic.FunctionalExtensionality.
 Require Import Classical.
+Require Import Bool.
+Require Import Classical.
 
 Parameter msg proc pst: Type.
 Parameter undefined : proc.
@@ -18,35 +20,41 @@ Inductive proc_state : Type :=
   | Aslept : proc_state.
 
 Record CHOAlgorith := {
-  CinitState : proc -> pst -> proc -> Prop;
+  Proc_set : set proc;
+  CinitState : proc -> pst -> proc -> bool;
   SendMsg : proc -> proc -> pst -> msg;
-  CnextState : proc -> pst -> (proc -> message) -> proc -> pst -> Prop }.
+  CnextState : proc -> pst -> (proc -> message) -> proc -> pst -> bool }.
 
-Definition initState alg p st : Prop := CinitState alg p st undefined.
+Definition initState alg p st : bool := CinitState alg p st undefined.
 Definition nextState alg p st msgs st' := CnextState alg p st msgs undefined st'.
 
 Definition HO := proc -> Ensemble proc.
 Definition coord := proc -> proc.
 
-Definition SHOmsgVectors A p cfg (HOp:set proc) SHOp :=
-  { mu : proc -> message | (forall q:proc, set_In q HOp <-> mu q <> Void) /\
+Definition SHOmsgVectors A p cfg HOp SHOp :=
+  { mu : proc -> message | (forall q, set_In q HOp <-> mu q <> Void) /\
       forall q, set_In q (set_inter proc_dec HOp SHOp) -> match cfg q with
   | Active s => mu q = Content (SendMsg A q p s)
   | _ => mu q = Bot end}.
 
-Definition CSHOnextConfig A cfg HO SHO coord cfg' : Prop :=
-   forall p, match cfg p with
+Definition forall_proc (A:CHOAlgorith) (f:proc -> bool) : bool :=
+  let fix forall_proc_ (l:set proc) f  := match l with
+  | nil => true
+  | cons a ar => andb (f a) (forall_proc_ ar f) end in forall_proc_ (Proc_set A) f. 
+
+Definition CSHOnextConfig A cfg HO SHO coord cfg' : bool :=
+   forall_proc A (fun p => match cfg p with
   | Active s => match cfg' p with
     | Active s' => exists mu : (SHOmsgVectors A p cfg (HO p) (SHO p)),
-           CnextState A p s (proj1_sig mu) (coord p) s'
+           CnextState A p s (proj1_sig mu) (coord p) s' = true
     | _ => False end
-  | _ => True end.
+  | _ => True end).
 
 Definition CHOinitConfig A rho coord :=
-  forall p : proc, exists n : nat, (forall m, m < n -> rho m p = Aslept) /\
+  forall_proc A (fun p => (exists n : nat, (forall m, m < n -> rho m p = Aslept) /\
   match rho n p with 
-  |Active s => CinitState A p s (coord n p)
-  | _ => False end.
+  |Active s => CinitState A p s (coord n p) = true
+  | _ => False end)).
 
 Definition CSHORun A rho HOs SHOs coords :=
   CHOinitConfig A rho coords
@@ -55,10 +63,10 @@ Definition CSHORun A rho HOs SHOs coords :=
 Definition HOinitConfig  A cfg := CHOinitConfig A cfg (fun _ _ => undefined).
 
 Lemma HOinitConfig_eq : forall A cfg, HOinitConfig A cfg =
-  forall p:proc, exists n:nat, (forall m, m < n -> cfg m p = Aslept) /\
+  forall_proc A (fun p => exists n:nat, (forall m, m < n -> cfg m p = Aslept) /\
   match cfg n p with 
-  |Active s => initState A p s
-  | _ => False end.
+  |Active s => initState A p s = true
+  | _ => False end).
 trivial.
 Qed.
 
@@ -70,7 +78,7 @@ Lemma SHOnextConfig_eq : forall A (cfg:proc->proc_state) HO SHO cfg',
     forall p,  match cfg p with
   | Active s => match cfg' p with
     | Active s' => exists mu : SHOmsgVectors A p cfg (HO p) (SHO p),
-        nextState A p s (proj1_sig mu) s'
+        nextState A p s (proj1_sig mu) s' = true
     | _ => False end
   | _ => True end.
 trivial.
@@ -122,7 +130,7 @@ Lemma CHOnextConfig_eq : forall A cfg HO coord cfg',
   CHOnextConfig A cfg HO coord cfg' =
   forall p,  match cfg p with
   | Active s => match cfg' p with
-    | Active s' => CnextState A p s (HOrcvMsgs A p (HO p) cfg) (coord p) s'
+    | Active s' => CnextState A p s (HOrcvMsgs A p (HO p) cfg) (coord p) s' = true
     | _ => False end
   | _ => True end.
 intros.
@@ -134,6 +142,15 @@ case (cfg x).
 intro.
 case (cfg' x).
 intro.
+
+induction (CnextState A x p (HOrcvMsgs A x (HO0 x) cfg) (coord0 x) p0).
+
+assert(H:=classic (exists mu : SHOmsgVectors A x cfg (HO0 x) (HO0 x),
+   CnextState A x p (proj1_sig mu) (coord0 x) p0 = true)).
+destruct H.
+destruct H.
+
+exists (HOrcvMsgs A x (HO0 x) cfg).
 unfold HOrcvMsgs.
 rewrite <- (SHOmsgVectors_HO.
 trivial.
